progress on array is sorted, but time to give up

resources/array_is_sorted/array_is_sorted_old.ml
@@ -2,10 +2,13 @@ open Combinators
 
 let array_is_sorted (t: int array) =
   let (len: int) = Array.length t in
-  let (res: bool option) = until_downto (len - 1) 0 (fun (i: int) ->
-    if t.(i -1) > t.(i)
-    then Some false
-    else None
-  ) in
-  let (res: bool) = not (Opt.option_is_some res) in
-  res
+  if len = 0
+  then true
+  else
+    let (res: unit option) = until_downto (len - 1) 0 (fun (i: int) ->
+      if t.(i -1) > t.(i)
+      then Some ()
+      else None
+    ) in
+    let (res: bool) = not (Opt.option_is_some res) in
+    res
