resources/array_is_sorted/Verify_array_is_sorted_old.v
@@ -4,27 +4,33 @@ From TLC Require Import LibListZ.
 
 From Common Require Import Verify_combinators Verify_opt.
 
-From Common Require Import Tactics.
-From Common Require Import Utils.
+From Common Require Import Tactics Utils Solver.
 
 From ProofsArrayIsSorted Require Import Array_is_sorted_old_ml.
 
-Definition is_sorted_internal ls :=
+Fixpoint is_sorted_internal_rec last_value ls :=
   match ls with
   | h :: t =>
-      is_some (List.fold_left
-                 (fun '(acc: option (bool * int)) (v: int) =>
-                    match acc with
-                    | None => None
-                    | Some (b, p_vl) =>
-                        if v <=? p_vl 
-                        then Some (true, v)
-                        else None
-                    end
-                 ) t (Some (true, h)))
+      if h <=? last_value
+      then is_sorted_internal_rec h t
+      else false
   | nil => true
   end.
-Definition is_sorted ls := is_sorted_internal (rev ls).
+
+Definition is_sorted ls :=
+  match ls with
+  | h :: t => is_sorted_internal_rec h t
+  | nil => true
+  end.
+
+Lemma is_sorted_internal_pres v ls :
+    is_sorted_internal_rec v ls = true ->
+    is_sorted ls = true.
+Proof.
+  case ls as [| x xs]; simpl; auto.
+  case (x <=? v); intro H; try inversion H; auto.
+Qed.
+
 
 Lemma array_is_sorted_spec :
   forall (a: array int) (l: list int),
@@ -34,17 +40,33 @@ Lemma array_is_sorted_spec :
 Proof using (All).
   xcf.
   xapp.
-  xletopaque tmp Htmp.
-  xapp (until_downto_spec (length l - 1) 0 tmp
-          (fun (i: int) (res: option bool) =>
-             a ~> Array l \*
-               \[res = res]
-          )
-       ). { admit. } { admit. } { admit. }
-  intros res i [Hi Himpl] Heq.
+  xif as Hcond.
+  - xvals*. { sis_list_solver. }
+  - xletopaque tmp Htmp.
+    xapp (until_downto_spec (length l - 1) 0 tmp
+            (fun (i: int) (res: option unit) =>
+               a ~> Array l \*
+                 \[res = opt_of_bool (negb (is_sorted (take (length l - i) (rev l))))]
+            )
+         ). {
+      sis_solve_start; sis_normalize_opt_of_bool; sis_normalize_boolean_goals.
+      gen H.
+      admit.
+      admit.
+    } { math. } {
+      sis_normalize_opt_of_bool; sis_normalize_boolean_goals.
+      math_rewrite (length l - (length l - 1) = 0 + 1).
+      case (rev l); [ | intros h t ]; rewrite ?take_nil, ?take_cons_pos; auto; try math.
+    }
+  intros res i Hterm Heq.
   xapp (opt_is_some_spec).
   xlet.
   xvals*. {
+    gen Hterm; subst; sis_normalize_opt_of_bool;
+      rewrite Bool.negb_involutive; intros Hterm.
+    rewrite <- negb_eq_neg, Bool.negb_involutive.
+    case_eq (is_sorted (take (length l - i) (rev l))).
+
     admit.
   }
 Admitted.
